Added domset-based tautology checker. Substantial runtime improvement.

checker/builtins.ml
@@ -39,6 +39,8 @@ let string_of_ivars model = string_of_list (M.ivar_name model)
 (* Checker for a tautological clause. *)
 let tauto bnd cl =
   C_impl.check_tauto_bnd bnd (impl_clause_of_clause cl)
+let tauto_dbnd dbnd cl =
+  C_impl.check_tauto_dbnd dbnd (impl_clause_of_clause cl)
 
 let clause_subsumes cl_x cl_y =
   C_impl.check_clause (impl_clause_of_clause cl_x) (impl_clause_of_clause cl_y)
