checker/builtins.mli
@@ -2,4 +2,5 @@
 val register : unit -> unit
 
 val tauto : MTypes.bounds -> MTypes.clause -> bool
+val tauto_dbnd : Checker_impl.domset -> MTypes.clause -> bool
 val clause_subsumes : MTypes.clause -> MTypes.clause -> bool
